makefile
@@ -3,9 +3,18 @@
 # 	ocamlc -c export.mli
 # 	ocamlopt export.ml	If you need the mli file
 
+HiDavid:
+	ocamlc -i HiDavid.ml > HiDavid.mli
+	ocamlc -c HiDavid.mli
+	ocamlopt HiDavid.ml
+
 
 all :
 	ocamlmktop -o mine graphics.cma sample.ml
+
+cleanHi:
+	rm HiDavid.mli
+	rm HiDavid.o
 
 clean:
 	rm sample.cmi
